BtcVerified.lean
@@ -27,6 +27,7 @@ import BtcVerified.Block.Commitment
 import BtcVerified.Block.BlockHash
 import BtcVerified.Block.Chain
 import BtcVerified.Consensus.Limits
+import BtcVerified.Consensus.LockTime
 import BtcVerified.Consensus.TxContext
 import BtcVerified.Consensus.ScriptCheck
 import BtcVerified.Consensus.TxStateless
